IsaSAT: finish Propagation

Weidenbach_Book/IsaSAT_Propagate_Conflict_LLVM.thy
@@ -45,161 +45,101 @@ apply (annot_snat_const "TYPE (64)")
 lemma le_uint64_max_minus_4_uint64_max: \<open>a \<le> sint64_max - 4 \<Longrightarrow> Suc a < max_snat 64\<close>
   by (auto simp: sint64_max_def max_snat_def)
 
+definition cut_watch_list_heur2_inv where
+  \<open>cut_watch_list_heur2_inv L n = (\<lambda>(j, w, W). j \<le> w \<and> w \<le> n \<and> nat_of_lit L < length W)\<close>
+
+lemma cut_watch_list_heur2_alt_def:
+\<open>cut_watch_list_heur2 = (\<lambda>j w L (M, N, D, Q, W, oth). do {
+  ASSERT(j \<le> length (W ! nat_of_lit L) \<and> j \<le> w \<and> nat_of_lit L < length W \<and>
+     w \<le> length (W ! (nat_of_lit L)));
+  let n = length (W!(nat_of_lit L));
+  (j, w, W) \<leftarrow> WHILE\<^sub>T\<^bsup>cut_watch_list_heur2_inv L n\<^esup>
+    (\<lambda>(j, w, W). w < n)
+    (\<lambda>(j, w, W). do {
+      ASSERT(w < length (W!(nat_of_lit L)));
+      RETURN (j+1, w+1, W[nat_of_lit L := (W!(nat_of_lit L))[j := W!(nat_of_lit L)!w]])
+    })
+    (j, w, W);
+  ASSERT(j \<le> length (W ! nat_of_lit L) \<and> nat_of_lit L < length W);
+  let W = W[nat_of_lit L := take j (W ! nat_of_lit L)];
+  RETURN (M, N, D, Q, W, oth)
+})\<close>
+  unfolding cut_watch_list_heur2_inv_def  cut_watch_list_heur2_def
+  by auto
+
+lemma cut_watch_list_heur2I:
+  \<open>length (a1'd ! nat_of_lit baa) \<le> sint64_max - 4 \<Longrightarrow>
+       cut_watch_list_heur2_inv baa (length (a1'd ! nat_of_lit baa))
+        (a1'e, a1'f, a2'f) \<Longrightarrow>
+       a1'f < length_ll a2'f (nat_of_lit baa) \<Longrightarrow>
+       ez \<le> bba \<Longrightarrow>
+       Suc a1'e < max_snat 64\<close>
+  \<open>length (a1'd ! nat_of_lit baa) \<le> sint64_max - 4 \<Longrightarrow>
+       cut_watch_list_heur2_inv baa (length (a1'd ! nat_of_lit baa))
+        (a1'e, a1'f, a2'f) \<Longrightarrow>
+       a1'f < length_ll a2'f (nat_of_lit baa) \<Longrightarrow>
+       ez \<le> bba \<Longrightarrow>
+       Suc a1'f < max_snat 64\<close>
+  \<open>cut_watch_list_heur2_inv baa (length (a1'd ! nat_of_lit baa))
+        (a1'e, a1'f, a2'f) \<Longrightarrow> nat_of_lit baa < length a2'f\<close>
+  \<open>cut_watch_list_heur2_inv baa (length (a1'd ! nat_of_lit baa))
+        (a1'e, a1'f, a2'f) \<Longrightarrow> a1'f < length_ll a2'f (nat_of_lit baa) \<Longrightarrow>
+       a1'e < length (a2'f ! nat_of_lit baa)\<close>
+  by (auto simp: max_snat_def sint64_max_def cut_watch_list_heur2_inv_def length_ll_def)
+
 sepref_definition cut_watch_list_heur2_fast_code
   is \<open>uncurry3 cut_watch_list_heur2\<close>
   :: \<open>[\<lambda>(((j, w), L), S). length (watched_by_int S L) \<le> sint64_max-4]\<^sub>a
      sint64_nat_assn\<^sup>k *\<^sub>a sint64_nat_assn\<^sup>k *\<^sub>a unat_lit_assn\<^sup>k *\<^sub>a
      isasat_bounded_assn\<^sup>d \<rightarrow> isasat_bounded_assn\<close>
   supply [[goals_limit=1]] (* length_ll_def[simp] sint64_max_le_max_snat64[intro]
-    le_uint64_max_minus_4_uint64_max[dest]*)  unfolding cut_watch_list_heur2_def isasat_bounded_assn_def length_ll_def[symmetric]
+    le_uint64_max_minus_4_uint64_max[dest]*) cut_watch_list_heur2I[intro] length_ll_def[simp]
+  unfolding cut_watch_list_heur2_alt_def isasat_bounded_assn_def length_ll_def[symmetric]
     nth_rll_def[symmetric]
     op_list_list_take_alt_def[symmetric]
     op_list_list_upd_alt_def[symmetric]
   apply (annot_snat_const "TYPE (64)")
-  apply sepref_dbg_preproc
-  apply sepref_dbg_cons_init
-  apply sepref_dbg_id
-  apply sepref_dbg_monadify
-  apply sepref_dbg_opt_init
-apply sepref_dbg_trans_step
-apply sepref_dbg_trans_step
-apply sepref_dbg_trans_step
-apply sepref_dbg_trans_step
-apply sepref_dbg_trans_step
-apply sepref_dbg_trans_step
-apply sepref_dbg_trans_step
-apply sepref_dbg_trans_step
-apply sepref_dbg_trans_step
-apply sepref_dbg_trans_step
-apply sepref_dbg_trans_step
-apply sepref_dbg_trans_step
-apply sepref_dbg_trans_step
-apply sepref_dbg_trans_step
-apply sepref_dbg_trans_step
-apply sepref_dbg_trans_step
-apply sepref_dbg_trans_step
-apply sepref_dbg_trans_step
-apply sepref_dbg_trans_step
-apply sepref_dbg_trans_step
-apply sepref_dbg_trans_step
-apply sepref_dbg_trans_step
-apply sepref_dbg_trans_step
-apply sepref_dbg_trans_step
-apply sepref_dbg_trans_step
-apply sepref_dbg_trans_step
-apply sepref_dbg_trans_step
-apply sepref_dbg_trans_step
-apply sepref_dbg_trans_step
-apply sepref_dbg_trans_step
-apply sepref_dbg_trans_step
-apply sepref_dbg_trans_step
-apply sepref_dbg_trans_step
-apply sepref_dbg_trans_step
-apply sepref_dbg_trans_step
-apply sepref_dbg_trans_step
-apply sepref_dbg_trans_step
-apply sepref_dbg_trans_step
-apply sepref_dbg_trans_step
-apply sepref_dbg_trans_step
-apply sepref_dbg_trans_step
-apply sepref_dbg_trans_step
-apply sepref_dbg_trans_step
-apply sepref_dbg_trans_step
-apply sepref_dbg_trans_step
-apply sepref_dbg_trans_step
-apply sepref_dbg_trans_step
-apply sepref_dbg_trans_step
-supply sint64_max_le_max_snat64[intro del:]
-    le_uint64_max_minus_4_uint64_max[dest del:]
-apply sepref_dbg_trans_step
-apply sepref_dbg_side
-apply sepref_dbg_trans_step
-apply sepref_dbg_trans_step
-apply sepref_dbg_trans_step
-apply sepref_dbg_trans_step
-apply sepref_dbg_trans_step
-apply sepref_dbg_trans_step
-apply sepref_dbg_trans_step
-apply sepref_dbg_trans_step
-apply sepref_dbg_trans_step
-apply sepref_dbg_trans_step
-apply sepref_dbg_trans_step
-apply sepref_dbg_trans_step
-apply sepref_dbg_trans_step
-apply sepref_dbg_trans_step
-apply sepref_dbg_trans_step
-apply sepref_dbg_trans_step
-apply sepref_dbg_trans_step
-apply sepref_dbg_trans_step
-apply sepref_dbg_trans_step
-apply sepref_dbg_trans_step
-apply sepref_dbg_trans_step
-
-oops
-  apply sepref_dbg_trans
-  apply sepref_dbg_opt
-  apply sepref_dbg_cons_solve
-  apply sepref_dbg_cons_solve
-  apply sepref_dbg_constraints
-
-  apply sepref_dbg_keep
-apply sepref_dbg_trans_keep
-apply sepref_dbg_trans_step_keep
-apply sepref_dbg_side_unfold
-subgoal
-apply (auto intro: sint64_max_le_max_snat64 simp: dest: le_uint64_max_minus_4_uint64_max )[]
-oops
   by sepref
 
 declare cut_watch_list_heur2_fast_code.refine[sepref_fr_rules]
-
+  unit_propagation_inner_loop_wl_loop_D_fast.refine[sepref_fr_rules]
 
 sepref_definition unit_propagation_inner_loop_wl_D_fast_code
   is \<open>uncurry unit_propagation_inner_loop_wl_D_heur\<close>
-  :: \<open>[\<lambda>(L, S). length (get_clauses_wl_heur S) \<le> uint64_max]\<^sub>a
+  :: \<open>[\<lambda>(L, S). length (get_clauses_wl_heur S) \<le> sint64_max]\<^sub>a
         unat_lit_assn\<^sup>k *\<^sub>a isasat_bounded_assn\<^sup>d \<rightarrow> isasat_bounded_assn\<close>
-  supply [[goals_limit=1]] nat_of_uint64_conv_hnr[sepref_fr_rules]
+  supply [[goals_limit=1]]
   unfolding PR_CONST_def unit_propagation_inner_loop_wl_D_heur_def
   by sepref
 
 declare unit_propagation_inner_loop_wl_D_fast_code.refine[sepref_fr_rules]
 
-
-sepref_definition select_and_remove_from_literals_to_update_wl_code
-  is \<open>select_and_remove_from_literals_to_update_wl_heur\<close>
-  :: \<open>isasat_unbounded_assn\<^sup>d \<rightarrow>\<^sub>a isasat_unbounded_assn *a unat_lit_assn\<close>
-  supply [[goals_limit=1]] uint32_nat_assn_plus[sepref_fr_rules]
-  unfolding select_and_remove_from_literals_to_update_wl_heur_alt_def isasat_unbounded_assn_def
-    one_uint32_nat_def[symmetric]
-  supply [[goals_limit = 1]]
+sepref_definition isa_trail_nth_fast_code
+  is \<open>uncurry isa_trail_nth\<close>
+  :: \<open>trail_pol_fast_assn\<^sup>k *\<^sub>a sint64_nat_assn\<^sup>k \<rightarrow>\<^sub>a unat_lit_assn\<close>
+  unfolding isa_trail_nth_def trail_pol_fast_assn_def
   by sepref
 
-declare select_and_remove_from_literals_to_update_wl_code.refine[sepref_fr_rules]
-
+declare isa_trail_nth_fast_code.refine[sepref_fr_rules]
+sepref_register isa_trail_nth
 sepref_definition select_and_remove_from_literals_to_update_wlfast_code
   is \<open>select_and_remove_from_literals_to_update_wl_heur\<close>
   :: \<open>isasat_bounded_assn\<^sup>d \<rightarrow>\<^sub>a isasat_bounded_assn *a unat_lit_assn\<close>
-  supply [[goals_limit=1]] uint32_nat_assn_plus[sepref_fr_rules]
+  supply [[goals_limit=1]]
   unfolding select_and_remove_from_literals_to_update_wl_heur_alt_def isasat_bounded_assn_def
-    one_uint32_nat_def[symmetric]
   supply [[goals_limit = 1]]
+  apply (annot_snat_const "TYPE (64)")
   by sepref
+
+find_theorems isa_trail_nth
+thm isa_trail_nth_fast_code.refine_raw
+
 
 declare select_and_remove_from_literals_to_update_wlfast_code.refine[sepref_fr_rules]
 
-
-sepref_definition literals_to_update_wl_literals_to_update_wl_empty_code
-  is \<open>RETURN o literals_to_update_wl_literals_to_update_wl_empty\<close>
-  :: \<open>[\<lambda>S. isa_length_trail_pre (get_trail_wl_heur S)]\<^sub>a isasat_unbounded_assn\<^sup>k \<rightarrow> bool_assn\<close>
-  unfolding literals_to_update_wl_literals_to_update_wl_empty_alt_def
-    isasat_unbounded_assn_def
-  by sepref
-
-declare literals_to_update_wl_literals_to_update_wl_empty_code.refine[sepref_fr_rules]
-
 sepref_definition literals_to_update_wl_literals_to_update_wl_empty_fast_code
   is \<open>RETURN o literals_to_update_wl_literals_to_update_wl_empty\<close>
-  :: \<open>[\<lambda>S. isa_length_trail_pre (get_trail_wl_heur S)]\<^sub>a isasat_bounded_assn\<^sup>k \<rightarrow> bool_assn\<close>
+  :: \<open>[\<lambda>S. isa_length_trail_pre (get_trail_wl_heur S)]\<^sub>a isasat_bounded_assn\<^sup>k \<rightarrow> bool1_assn\<close>
   unfolding literals_to_update_wl_literals_to_update_wl_empty_alt_def
     isasat_bounded_assn_def
   by sepref
@@ -210,20 +150,17 @@ sepref_register literals_to_update_wl_literals_to_update_wl_empty
   select_and_remove_from_literals_to_update_wl_heur
 
 
-sepref_definition unit_propagation_outer_loop_wl_D_code
-  is \<open>unit_propagation_outer_loop_wl_D_heur\<close>
-  :: \<open>isasat_unbounded_assn\<^sup>d \<rightarrow>\<^sub>a isasat_unbounded_assn\<close>
-  supply [[goals_limit=1]]
-    unit_propagation_outer_loop_wl_D_invI[intro]
-  unfolding unit_propagation_outer_loop_wl_D_heur_def
-    literals_to_update_wl_literals_to_update_wl_empty_def[symmetric]
-  by sepref
-
-declare unit_propagation_outer_loop_wl_D_code.refine[sepref_fr_rules]
+lemma unit_propagation_outer_loop_wl_D_heur_fast:
+  \<open>length (get_clauses_wl_heur x) \<le> sint64_max \<Longrightarrow>
+       unit_propagation_outer_loop_wl_D_heur_inv x s' \<Longrightarrow>
+       length (get_clauses_wl_heur a1') =
+       length (get_clauses_wl_heur s') \<Longrightarrow>
+       length (get_clauses_wl_heur s') \<le> sint64_max\<close>
+  by (auto simp: unit_propagation_outer_loop_wl_D_heur_inv_def)
 
 sepref_definition unit_propagation_outer_loop_wl_D_fast_code
   is \<open>unit_propagation_outer_loop_wl_D_heur\<close>
-  :: \<open>[\<lambda>S. length (get_clauses_wl_heur S) \<le> uint64_max]\<^sub>a isasat_bounded_assn\<^sup>d \<rightarrow> isasat_bounded_assn\<close>
+  :: \<open>[\<lambda>S. length (get_clauses_wl_heur S) \<le> sint64_max]\<^sub>a isasat_bounded_assn\<^sup>d \<rightarrow> isasat_bounded_assn\<close>
   supply [[goals_limit=1]] unit_propagation_outer_loop_wl_D_heur_fast[intro]
     unit_propagation_outer_loop_wl_D_invI[intro]
   unfolding unit_propagation_outer_loop_wl_D_heur_def
